trunk/source/LTL2aut/src/de/uni_freiburg/informatik/ultimate/LTL2aut/DummyLTL2autObserver.java
@@ -4,7 +4,10 @@ import java.io.BufferedReader;
 import java.io.FileReader;
 import java.io.IOException;
 import java.io.InputStreamReader;
+import java.util.ArrayList;
+import java.util.Arrays;
 import java.util.HashMap;
+import java.util.Map;
 
 import org.apache.commons.io.IOUtils;
 import org.apache.log4j.Logger;
@@ -17,6 +20,7 @@ import de.uni_freiburg.informatik.ultimate.access.WalkerOptions;
 import de.uni_freiburg.informatik.ultimate.core.api.UltimateServices;
 import de.uni_freiburg.informatik.ultimate.core.preferences.UltimatePreferenceStore;
 import de.uni_freiburg.informatik.ultimate.model.IElement;
+import de.uni_freiburg.informatik.ultimate.model.boogie.ast.Unit;
 
 /**
  * This class reads a definition of a property in ltl and returns the AST of the
@@ -29,75 +33,105 @@ public class DummyLTL2autObserver implements IUnmanagedObserver {
 
 	private AstNode mRootNode;
 	private Logger mLogger;
+	private String mInputFile;
+
+	private static final String sLTLMarker = "#LTLProperty:";
+	private static final String sIRSMarker = "#IRS:";
 
 	@Override
 	public void init() {
 		mLogger = UltimateServices.getInstance().getLogger(Activator.PLUGIN_ID);
 		mRootNode = null;
+		mInputFile = null;
 	}
 
 	@Override
 	public void finish() throws Throwable {
-		AstNode node;
-		String line;
+		String[] specification = getSpecification();
+		AstNode node = getProperty(specification[0]);
+		Map<String, AstNode> irs = getIRS(Arrays.copyOfRange(specification, 1, specification.length));
+		new SubstituteAPVisitor(irs, node);
+		mRootNode = node;
+	}
 
+	private String[] getSpecification() throws IOException {
+		if (PreferenceInitializer.readPropertyFromFile()) {
+			if (mInputFile != null) {
+				BufferedReader br;
+				String line = null;
+				ArrayList<String> properties = new ArrayList<>();
+				ArrayList<String> irs = new ArrayList<>();
+				try {
+					br = new BufferedReader(new FileReader(mInputFile));
+					while ((line = br.readLine()) != null) {
+						if (line.contains(sLTLMarker)) {
+							properties.add(line.replaceFirst("//", "").replaceAll(sLTLMarker, "").trim());
+						}
+						if (line.contains(sIRSMarker)) {
+							irs.add(line.replaceFirst("//", "").replaceAll(sIRSMarker, "").trim());
+						}
+					}
+					br.close();
+				} catch (IOException e) {
+					mLogger.error("Error while reading " + mInputFile + ": " + e);
+					line = null;
+					throw e;
+				}
+
+				if (properties.isEmpty()) {
+					mLogger.info("No LTL specification in input file.");
+				} else {
+					if (properties.size() > 1) {
+						throw new UnsupportedOperationException("We currently support only 1 LTL property at a time.");
+					}
+					String[] rtr = new String[1 + irs.size()];
+					rtr[0] = properties.get(0);
+					int i = 1;
+					for (String entry : irs) {
+						rtr[i] = entry;
+						i++;
+					}
+					return rtr;
+				}
+			}
+		}
+
+		mLogger.info("Using LTL specification from settings.");
 		String property = new UltimatePreferenceStore(Activator.PLUGIN_ID)
 				.getString(PreferenceInitializer.LABEL_PPROPERTY);
+		return property.split("\n");
 
-		// BufferedReader br;
-		// String line = null;
-		// try {
-		// br = new BufferedReader(new FileReader(inputFile));
-		// line = br.readLine();
-		// br.close();
-		// } catch (IOException e) {
-		// line = null;
-		// }
+	}
 
-		BufferedReader br = new BufferedReader(new InputStreamReader(IOUtils.toInputStream(property)));
+	private AstNode getProperty(String property) throws Throwable {
 		try {
-			// read the LTL formula from the first line and pass it to the
-			// parser
-			line = br.readLine();
-
-			// translate to ba with external tool and get AST
-			WrapLTL2Never wrap = new WrapLTL2Never();
-			node = wrap.ltl2Ast(line);
+			mLogger.debug("Parsing LTL property...");
+			return new WrapLTL2Never().ltl2Ast(property);
 		} catch (Throwable e) {
 			mLogger.error(String.format("Exception during LTL->BA execution: %s", e));
 			throw e;
 		}
+	}
 
-		try {
-			// Read following lines and get Atomic Props
-			HashMap<String, AstNode> aps = new HashMap<String, AstNode>(); // ident
-																			// ->
-																			// propostition
-			line = br.readLine();
-			while (line != null) {
-				LexerAP lexer = new LexerAP(new InputStreamReader(IOUtils.toInputStream(line)));
+	private Map<String, AstNode> getIRS(String[] entries) throws Throwable {
+		mLogger.debug("Parsing mapping from AP to boolean expression over program variables...");
+		Map<String, AstNode> aps = new HashMap<String, AstNode>();
+		for (String entry : entries) {
+			try {
+				LexerAP lexer = new LexerAP(new InputStreamReader(IOUtils.toInputStream(entry.trim())));
 				ParserAP p = new ParserAP(lexer);
-				mLogger.debug("Parsing LTL property...");
+
 				AstNode nodea = (AstNode) p.parse().value;
 				// append node to dictionary of atomic propositions
-				if (nodea instanceof AtomicProposition)
+				if (nodea instanceof AtomicProposition) {
 					aps.put(((AtomicProposition) nodea).getIdent(), nodea.getOutgoingNodes().get(0));
-
-				line = br.readLine();
+				}
+			} catch (Throwable e) {
+				mLogger.error(String.format("Exception while parsing the atomic proposition \"%s\": %s", entry, e));
+				throw e;
 			}
-			// substitute props in AST
-			new SubstituteAPVisitor(aps, node);
-
-			mRootNode = node;
-
-		} catch (Throwable e) {
-			if (line != null) {
-				mLogger.error(String.format("Exception while parsing the atomic proposition \"%s\": %s", line, e));
-			} else {
-				mLogger.error(String.format("Exception while parsing the atomic propositions: %s", e));
-			}
-			throw e;
 		}
+		return aps;
 	}
 
 	@Override
@@ -112,6 +146,9 @@ public class DummyLTL2autObserver implements IUnmanagedObserver {
 
 	@Override
 	public boolean process(IElement root) throws Throwable {
+		if (root instanceof Unit) {
+			mInputFile = ((Unit) root).getLocation().getFileName();
+		}
 		return false;
 	}
 
